src/dvspec/dafny/att_spec_proofs/incomplete_proofs.dfy
@@ -23,16 +23,12 @@ module Incomplete_Proofs
     import opened DVN_Next_Inv
     import opened Fnc_Inv    
 
-        
+    lemma {:axiom} axiom_inv10(dvc: DVCNodeState)    
+    ensures inv10_body(dvc)
+
+    
+    
     
 
     
-
-       
-
-    
-
-    
-
-         
 }
